wip: tried to put pmi and fr directly into context resource

fairness/examples/comp/comp_lib_pmp.v
@@ -18,8 +18,10 @@ Close Scope Z_scope.
 Section LibPMP. 
   Context `{EM: ExecutionModel heap_lang M} `{@heapGS Σ _ EM} {cpG: clientPreGS Σ}.
   Context `{PMPP: @PartialModelPredicatesPre (locale heap_lang) _ _ Σ client_model_impl}.
+  Context {relies_on_cl: locale heap_lang -> locale heap_lang -> iProp Σ}. 
+  Notation " τ '⤞_cl' g" := (relies_on_cl τ g) (at level 20). 
 
-  Notation "'LSG' Einvs" := (LM_steps_gen Einvs (EM := EM) (iLM := client_model) (PMPP := PMPP) (eGS := heap_fairnessGS)) (at level 10).
+  Notation "'LSG' Einvs" := (LM_steps_gen Einvs (EM := EM) (iLM := client_model) (PMPP := PMPP) (eGS := heap_fairnessGS) (relies_on := relies_on_cl)) (at level 10).
 
   Tactic Notation "specialize_full" ident(H) :=
     let foo := fresh in
@@ -31,31 +33,32 @@ Section LibPMP.
     done.
   Qed. 
 
-  Lemma update_client_state `{clientGS Σ} Einvs
+  Lemma update_client_state `{clientGS Σ} tid Einvs
     (extr: execution_trace heap_lang) (mtr: auxiliary_trace M)
     c2 (lb lb': fmstate lf) f
     (LIB_STEP: locale_trans lb ρlg lb' (LM := lib_model lib_gs))
-    (PROG_STEP: locale_step (trace_last extr) (Some 0) c2)
+    (PROG_STEP: locale_step (trace_last extr) (Some tid) c2)
     (F_BOUND: f ≤ client_fl)
     :
     LSG Einvs ⊢
     em_msi (trace_last extr) (trace_last mtr) (em_GS0 := heap_fairnessGS) -∗
     partial_model_is (lb, 1) -∗
     partial_free_roles_are {[ρ_cl]} -∗
-    has_fuels 0 {[ρ_lib := f]}
+    tid ⤞_cl tid -∗
+    has_fuels tid {[ρ_lib := f]}
     ={Einvs}=∗
     ∃ (δ2 : M) (ℓ: mlabel M),
-      ⌜em_valid_evolution_step (Some 0) c2 (trace_last mtr) ℓ δ2⌝ ∗
+      ⌜em_valid_evolution_step (Some tid) c2 (trace_last mtr) ℓ δ2⌝ ∗
       em_msi c2 δ2 (em_GS0 := heap_fairnessGS) ∗
-      has_fuels 0 (if decide (ls_tmap lb' !! ρlg = Some ∅)
+      tid ⤞_cl tid ∗
+      has_fuels tid (if decide (ls_tmap lb' !! ρlg = Some ∅)
                    then {[ρ_cl := client_fl]}
                    else {[ρ_lib := f]}) ∗
       partial_model_is (lb', 1) ∗
       partial_free_roles_are
       (if decide (ls_tmap lb' !! ρlg = Some ∅) then {[ρ_lib]} else {[ρ_cl]}).
-  Proof.
-    
-    iIntros "#PMP MSI ST FR FUELS".
+  Proof.    
+    iIntros "#PMP MSI ST FR RON FUELS".
     Local Ltac dEq := destruct (decide (_ = _)).
     Local Ltac dEl := destruct (decide (_ ∈ _)).
     pose proof (LM_map_empty_notlive lb' ρlg (LF := (@lib_LF _ lib_gs_ne))).
@@ -69,7 +72,7 @@ Section LibPMP.
     destruct c2 as (σ2, tp2).
 
     iPoseProof (LM_steps_gen_nofork_sub with "PMP") as "PMP'". 
-    iPoseProof (update_step_still_alive_gen with "[$] [$] [$] [$] [$]") as "EM_STEP".
+    iPoseProof (update_step_still_alive_gen with "[$] [$] [$] [$] [$] [$]") as "EM_STEP".
     7: { apply PROG_STEP. }
     7: { apply ct_lib_step. simpl. eauto. }
     { rewrite LIVE LIVE'.
@@ -120,7 +123,7 @@ Section LibPMP.
       by rewrite lookup_insert dom_singleton_L. }
       
     rewrite LIVE LIVE'.
-    iMod "EM_STEP" as (??) "(?&?&?&?&FREE)".
+    iMod "EM_STEP" as (??) "(?&?&?&?&?&FREE)".
     iModIntro. do 2 iExists _. iFrame.
     
     iApply partial_free_roles_are_Proper; [| iFrame].
@@ -147,26 +150,15 @@ Section LibPMP.
     - iModIntro. iFrame.
   Qed.
      
-
-  (* TODO: remove tid=0 restriction ? *)
-  Let lib_pmi `{clientGS Σ} (m: gmap (locale heap_lang) (gset (fmrole lib_model_impl))): iProp Σ:=
-    (∃ (L: gset (fmrole lib_model_impl)) (Ract Rfr: gset client_role),
-        ⌜ m = {[ 0 := L ]} ⌝ ∗
-         frag_mapping_is {[ ρlg := L ]} ∗
-         (⌜ L ≠ ∅ ⌝ ∗ ⌜ Ract = {[ ρ_lib ]} /\ Rfr = {[ ρ_cl ]} ⌝ ∗ (∃ f: nat, partial_fuel_is {[ ρ_lib := f ]} ∗ ⌜ 1 <= f <= client_fl ⌝) ∨
-          ⌜ L = ∅ ⌝ ∗ ⌜ Ract = {[ ρ_cl ]} /\ Rfr = {[ ρ_lib ]} ⌝ ∗ partial_fuel_is {[ inr ρy := client_fl ]}) ∗
-        partial_mapping_is {[ 0 := Ract ]} ∗
-        partial_free_roles_are Rfr ∗
-        y_frag_model_is 1).
   
   Definition lib_PMPP `{clientGS Σ}:
-    @PartialModelPredicatesPre (locale heap_lang) _ _ Σ lib_model_impl.
+    @PartialModelPredicatesPre lib_grole _ _ Σ lib_model_impl.
    refine
     {|
         partial_model_is := frag_model_is;
         partial_free_roles_are := frag_free_roles_are;
         partial_fuel_is := frag_fuel_is;
-        partial_mapping_is := lib_pmi;
+        partial_mapping_is := partial_mapping_is;
     |}.
   Unshelve.
   all: try (apply _ || solve_proper).
@@ -182,353 +174,384 @@ Section LibPMP.
   - iApply own_unit.
   Defined.
 
-  Lemma lib_open_inv `{clientGS Σ} ζ fs (FSnz : fs ≠ ∅):
-    client_inv -∗ has_fuels ζ fs (PMPP := lib_PMPP) -∗
-    |={↑Ns, ∅}=>
-    ⌜ ζ = 0 ⌝ ∗
-    (∃ lb, partial_model_is (lb, 1) (PartialModelPredicatesPre := PMPP) ∗ model_state_interp lb) ∗
-    frag_mapping_is {[ρlg := dom fs]}  ∗ y_auth_model_is 1 ∗
-    (∃ f, partial_fuel_is {[ρ_lib := f]} ∗ ⌜ 1 <= f <= client_fl ⌝) ∗
-    partial_mapping_is {[0 := {[ρ_lib]}]} ∗
-    partial_free_roles_are {[inr ρy]} ∗ y_frag_model_is 1 ∗
-    frag_fuel_is fs ∗
-    (▷ (∃ st, client_inv_impl st) ={ ∅, ↑Ns}=∗ emp).
-  Proof.
-    iIntros "#INV FUELS_LIB".
-    iInv Ns as ((lb, y)) ">(ST & YST_AUTH & inv')" "CLOS".
-    rewrite difference_diag_L. iModIntro.
-    iDestruct (has_fuels_equiv with "FUELS_LIB") as "[MAP_LIB FUEL_LIB]".
-    simpl. iDestruct "MAP_LIB" as (???) "(%LIBM&LM&MATCH&MAP&FR&YST)".
-    assert (ζ = 0 /\ L = dom fs) as [-> ->]; [| clear LIBM].
-    { by apply map_singleton_inj in LIBM as [-> <-]. }
-    (* assert (S <$> fs ≠ ∅) by (by intros ?%fmap_empty_inv). *)
-    iDestruct "MATCH" as "[(_&[-> ->]&(%f & Ff & %BOUND)) | [% _]]".
-    2: { exfalso. apply FSnz. apply dom_empty_iff. set_solver. }
-    iPoseProof (y_model_agree with "YST_AUTH YST") as "->".
-    iPoseProof (frag_mapping_same with "[inv'] LM") as "%TMAP0".
-    { iDestruct "inv'" as (?)"(?&?&?)". iFrame. }
-    iPoseProof (frag_fuel_included with "[inv'] [FUEL_LIB]") as "%FUEL0".
-    { iDestruct "inv'" as (?)"(?&?&?&?)". iFrame. }
-    { iApply frag_fuel_is_big_sepM; [done | by iFrame]. }
-    iSplitR; [done| ].
-    iFrame. iSplitL "ST inv'".
-    - iExists lb. iFrame. 
-    - iDestruct (frag_fuel_is_big_sepM with "FUEL_LIB") as "?"; [done| ].
-      iFrame. iExists _. iFrame. done.
-  Qed.
+  (* Let lib_pmi `{clientGS Σ} (m: gmap (locale heap_lang) (gset (fmrole lib_model_impl))): iProp Σ:= *)
+  (*   (∃ (L: gset (fmrole lib_model_impl)) (Ract Rfr: gset client_role), *)
+  (*       ⌜ m = {[ 0 := L ]} ⌝ ∗ *)
+  (*        frag_mapping_is {[ ρlg := L ]} ∗ *)
+  (*        (⌜ L ≠ ∅ ⌝ ∗ ⌜ Ract = {[ ρ_lib ]} /\ Rfr = {[ ρ_cl ]} ⌝ ∗ (∃ f: nat, partial_fuel_is {[ ρ_lib := f ]} ∗ ⌜ 1 <= f <= client_fl ⌝) ∨ *)
+  (*         ⌜ L = ∅ ⌝ ∗ ⌜ Ract = {[ ρ_cl ]} /\ Rfr = {[ ρ_lib ]} ⌝ ∗ partial_fuel_is {[ inr ρy := client_fl ]}) ∗ *)
+  (*       partial_mapping_is {[ 0 := Ract ]} ∗ *)
+  (*       partial_free_roles_are Rfr ∗ *)
+  (*       y_frag_model_is 1). *)
+
+  Definition relies_on_lib `{clientGS Σ} (τ: locale heap_lang) (g: lib_grole): iProp Σ :=
+    (∃ (Ract Rfr: gset client_role),
+        (* ⌜ m = {[ 0 := L ]} ⌝ ∗ *)
+         (* frag_mapping_is {[ ρlg := L ]} ∗ *)
+         (
+            (* ⌜ L ≠ ∅ ⌝ ∗ *)
+            ⌜ Ract = {[ ρ_lib ]} /\ Rfr = {[ ρ_cl ]} ⌝ ∗ (∃ f: nat, partial_fuel_is {[ ρ_lib := f ]} ∗ ⌜ 1 <= f <= client_fl ⌝) ∨
+          (* ⌜ L = ∅ ⌝ ∗ *)
+          ⌜ Ract = {[ ρ_cl ]} /\ Rfr = {[ ρ_lib ]} ⌝ ∗ partial_fuel_is {[ inr ρy := client_fl ]}) ∗
+
+        partial_mapping_is {[ τ := Ract ]} ∗ 
+        τ ⤞_cl τ ∗
+
+        partial_free_roles_are Rfr ∗
+        y_frag_model_is 1).
+        
+
+  
+  (* TODO: restore proofs below;
+     try to write a universal one covering any allowed lib proof rule *)
+  
+  (* Lemma lib_open_inv `{clientGS Σ} ζ fs (FSnz : fs ≠ ∅): *)
+  (*   client_inv -∗ has_fuels ζ fs (PMPP := lib_PMPP) -∗ *)
+  (*   |={↑Ns, ∅}=> *)
+  (*   ⌜ ζ = 0 ⌝ ∗ *)
+  (*   (∃ lb, partial_model_is (lb, 1) (PartialModelPredicatesPre := PMPP) ∗ model_state_interp lb) ∗ *)
+  (*   frag_mapping_is {[ρlg := dom fs]}  ∗ y_auth_model_is 1 ∗ *)
+  (*   (∃ f, partial_fuel_is {[ρ_lib := f]} ∗ ⌜ 1 <= f <= client_fl ⌝) ∗ *)
+  (*   partial_mapping_is {[0 := {[ρ_lib]}]} ∗ *)
+  (*   partial_free_roles_are {[inr ρy]} ∗ y_frag_model_is 1 ∗ *)
+  (*   frag_fuel_is fs ∗ *)
+  (*   (▷ (∃ st, client_inv_impl st) ={ ∅, ↑Ns}=∗ emp). *)
+  (* Proof. *)
+  (*   iIntros "#INV FUELS_LIB". *)
+  (*   iInv Ns as ((lb, y)) ">(ST & YST_AUTH & inv')" "CLOS". *)
+  (*   rewrite difference_diag_L. iModIntro. *)
+  (*   iDestruct (has_fuels_equiv with "FUELS_LIB") as "[MAP_LIB FUEL_LIB]". *)
+  (*   simpl. iDestruct "MAP_LIB" as (???) "(%LIBM&LM&MATCH&MAP&FR&YST)". *)
+  (*   assert (ζ = 0 /\ L = dom fs) as [-> ->]; [| clear LIBM]. *)
+  (*   { by apply map_singleton_inj in LIBM as [-> <-]. } *)
+  (*   (* assert (S <$> fs ≠ ∅) by (by intros ?%fmap_empty_inv). *) *)
+  (*   iDestruct "MATCH" as "[(_&[-> ->]&(%f & Ff & %BOUND)) | [% _]]". *)
+  (*   2: { exfalso. apply FSnz. apply dom_empty_iff. set_solver. } *)
+  (*   iPoseProof (y_model_agree with "YST_AUTH YST") as "->". *)
+  (*   iPoseProof (frag_mapping_same with "[inv'] LM") as "%TMAP0". *)
+  (*   { iDestruct "inv'" as (?)"(?&?&?)". iFrame. } *)
+  (*   iPoseProof (frag_fuel_included with "[inv'] [FUEL_LIB]") as "%FUEL0". *)
+  (*   { iDestruct "inv'" as (?)"(?&?&?&?)". iFrame. } *)
+  (*   { iApply frag_fuel_is_big_sepM; [done | by iFrame]. } *)
+  (*   iSplitR; [done| ]. *)
+  (*   iFrame. iSplitL "ST inv'". *)
+  (*   - iExists lb. iFrame.  *)
+  (*   - iDestruct (frag_fuel_is_big_sepM with "FUEL_LIB") as "?"; [done| ]. *)
+  (*     iFrame. iExists _. iFrame. done. *)
+  (* Qed. *)
 
 
-  Lemma fuel_keep_step_lifting `{clientGS Σ} Einvs (DISJ_INV: Einvs ## ↑Ns):
-  LSG Einvs ∗ client_inv ⊢
-  ∀ (extr : execution_trace heap_lang) (auxtr : auxiliary_trace M)
-    (c2 : cfg heap_lang) (fs : gmap (fmrole lib_model_impl) nat)
-    (ζ : locale heap_lang) (_ : dom fs ≠ ∅) (_ : locale_step
-                                                   (trace_last extr)
-                                                   (Some ζ) c2),
-    has_fuels ζ (S <$> fs) (PMPP := lib_PMPP) -∗
-    em_msi (trace_last extr) (trace_last auxtr) (em_GS0 := heap_fairnessGS)
-    ={Einvs ∪ ↑Ns}=∗
-    ∃ (δ2 : M) (ℓ : mlabel M),
-      ⌜em_valid_state_evolution_fairness (extr :tr[ Some ζ ]: c2)
-         (auxtr :tr[ ℓ ]: δ2)⌝ ∗
-      has_fuels ζ (filter (λ '(k, _), k ∈ dom fs ∖ ∅) fs) (PMPP := lib_PMPP) ∗
-      em_msi c2 δ2 (em_GS0 := heap_fairnessGS).
-  Proof.
-    iIntros "[#PMP #COMP]". iIntros "* FUELS_LIB MSI". simpl in *.
+  (* Lemma fuel_keep_step_lifting `{clientGS Σ} Einvs (DISJ_INV: Einvs ## ↑Ns): *)
+  (* LSG Einvs ∗ client_inv ⊢ *)
+  (* ∀ (extr : execution_trace heap_lang) (auxtr : auxiliary_trace M) *)
+  (*   (c2 : cfg heap_lang) (fs : gmap (fmrole lib_model_impl) nat) *)
+  (*   (ζ : locale heap_lang) (_ : dom fs ≠ ∅) (_ : locale_step *)
+  (*                                                  (trace_last extr) *)
+  (*                                                  (Some ζ) c2), *)
+  (*   has_fuels ζ (S <$> fs) (PMPP := lib_PMPP) -∗ *)
+  (*   em_msi (trace_last extr) (trace_last auxtr) (em_GS0 := heap_fairnessGS) *)
+  (*   ={Einvs ∪ ↑Ns}=∗ *)
+  (*   ∃ (δ2 : M) (ℓ : mlabel M), *)
+  (*     ⌜em_valid_state_evolution_fairness (extr :tr[ Some ζ ]: c2) *)
+  (*        (auxtr :tr[ ℓ ]: δ2)⌝ ∗ *)
+  (*     has_fuels ζ (filter (λ '(k, _), k ∈ dom fs ∖ ∅) fs) (PMPP := lib_PMPP) ∗ *)
+  (*     em_msi c2 δ2 (em_GS0 := heap_fairnessGS). *)
+  (* Proof. *)
+  (*   iIntros "[#PMP #COMP]". iIntros "* FUELS_LIB MSI". simpl in *. *)
     
-    assert (S <$> fs ≠ ∅) as NE.
-    { intros ?%dom_empty_iff. set_solver. }
+  (*   assert (S <$> fs ≠ ∅) as NE. *)
+  (*   { intros ?%dom_empty_iff. set_solver. } *)
 
-    iPoseProof (lib_open_inv with "[$] FUELS_LIB") as "INV'"; [set_solver| ].
-    rewrite union_comm_L.
-    iMod (fupd_mask_frame_r _ _ Einvs with "INV'") as
-      "(-> & (%lb & ST & inv') & LM & YST_AUTH & (%f & Ff & %BOUND) & MAP & FR & YST & FUEL_LIB & CLOS)"; [set_solver| ].
+  (*   iPoseProof (lib_open_inv with "[$] FUELS_LIB") as "INV'"; [set_solver| ]. *)
+  (*   rewrite union_comm_L. *)
+  (*   iMod (fupd_mask_frame_r _ _ Einvs with "INV'") as *)
+  (*     "(-> & (%lb & ST & inv') & LM & YST_AUTH & (%f & Ff & %BOUND) & MAP & FR & YST & FUEL_LIB & CLOS)"; [set_solver| ]. *)
 
     
-    iMod (actual_update_no_step_enough_fuel_keep with "[LM FUEL_LIB] inv'") as (lb') "(%LIB_STEP & FUELS_LIB & MSI_LIB & %TMAP_LIB)".
-    (* 3: { apply empty_subseteq. } *)
-    { eauto. }
-    { clear. red. intros. done. }
-    { rewrite /has_fuels_S. rewrite has_fuels_equiv. iFrame.
-      iApply frag_fuel_is_big_sepM; done. }
+  (*   iMod (actual_update_no_step_enough_fuel_keep with "[LM FUEL_LIB] inv'") as (lb') "(%LIB_STEP & FUELS_LIB & MSI_LIB & %TMAP_LIB)". *)
+  (*   (* 3: { apply empty_subseteq. } *) *)
+  (*   { eauto. } *)
+  (*   { clear. red. intros. done. } *)
+  (*   { rewrite /has_fuels_S. rewrite has_fuels_equiv. iFrame. *)
+  (*     iApply frag_fuel_is_big_sepM; done. } *)
     
-    destruct (trace_last extr) as (σ1, tp1) eqn:LASTE. destruct c2 as (σ2, tp2).
-    rewrite LASTE.
-    rewrite difference_empty_L.
-    (* rewrite difference_empty_L in TMAP_LIB. *)
-    iAssert (has_fuels 0 {[ ρ_lib := f ]}) with "[MAP Ff]" as "FUELS".
-    { rewrite /has_fuels. rewrite dom_singleton_L big_sepS_singleton.
-      rewrite lookup_singleton. iFrame. iExists _. iFrame. done. }
+  (*   destruct (trace_last extr) as (σ1, tp1) eqn:LASTE. destruct c2 as (σ2, tp2). *)
+  (*   rewrite LASTE. *)
+  (*   rewrite difference_empty_L. *)
+  (*   (* rewrite difference_empty_L in TMAP_LIB. *) *)
+  (*   iAssert (has_fuels 0 {[ ρ_lib := f ]}) with "[MAP Ff]" as "FUELS". *)
+  (*   { rewrite /has_fuels. rewrite dom_singleton_L big_sepS_singleton. *)
+  (*     rewrite lookup_singleton. iFrame. iExists _. iFrame. done. } *)
 
-    rewrite -LASTE.
-    iPoseProof (update_client_state with "[$] [$] [$] [$] [$]") as "EM_STEP"; eauto.
-    { eexists. split; [apply LIB_STEP| ]. done. }
-    { lia. }
-    iMod (fupd_mask_mono with "EM_STEP") as (δ2 ℓ) "(EV & MSI & FUELS & ST & FR)"; [set_solver| ].
-    do 2 iExists _. iFrame "EV MSI".
-    rewrite gmap_filter_dom_id. 
+  (*   rewrite -LASTE. *)
+  (*   iPoseProof (update_client_state with "[$] [$] [$] [$] [$]") as "EM_STEP"; eauto. *)
+  (*   { eexists. split; [apply LIB_STEP| ]. done. } *)
+  (*   { lia. } *)
+  (*   iMod (fupd_mask_mono with "EM_STEP") as (δ2 ℓ) "(EV & MSI & FUELS & ST & FR)"; [set_solver| ]. *)
+  (*   do 2 iExists _. iFrame "EV MSI". *)
+  (*   rewrite gmap_filter_dom_id.  *)
 
-    iDestruct ("CLOS" with "[ST MSI_LIB YST_AUTH]") as "CLOS".
-    { iNext. iExists (_, _). rewrite /client_inv_impl. iFrame. }
-    iMod (fupd_mask_frame_r _ _ Einvs with "CLOS") as "_"; [set_solver| ].
+  (*   iDestruct ("CLOS" with "[ST MSI_LIB YST_AUTH]") as "CLOS". *)
+  (*   { iNext. iExists (_, _). rewrite /client_inv_impl. iFrame. } *)
+  (*   iMod (fupd_mask_frame_r _ _ Einvs with "CLOS") as "_"; [set_solver| ]. *)
 
-    iModIntro.
-    iDestruct "FUELS" as "[MAP FUEL]". iDestruct "FUELS_LIB" as "[MAP_LIB FUELS_LIB]".
-    rewrite /has_fuels. iSplitR "FUELS_LIB".
-    2: { done. }
-    simpl. 
-    rewrite /lib_pmi. do 3 iExists _. iFrame.
-    iSplitR; [done| ].
-    (* TODO: case when domain becomes empty *)
-    iLeft. iSplitR; [done| ].
-    rewrite TMAP_LIB.
-    (* rewrite lookup_insert. *)
+  (*   iModIntro. *)
+  (*   iDestruct "FUELS" as "[MAP FUEL]". iDestruct "FUELS_LIB" as "[MAP_LIB FUELS_LIB]". *)
+  (*   rewrite /has_fuels. iSplitR "FUELS_LIB". *)
+  (*   2: { done. } *)
+  (*   simpl.  *)
+  (*   rewrite /lib_pmi. do 3 iExists _. iFrame. *)
+  (*   iSplitR; [done| ]. *)
+  (*   (* TODO: case when domain becomes empty *) *)
+  (*   iLeft. iSplitR; [done| ]. *)
+  (*   rewrite TMAP_LIB. *)
+  (*   (* rewrite lookup_insert. *) *)
 
-    assert (ls_tmap lb !! ρlg ≠ Some ∅) as TM_NE.
-    { edestruct (locale_trans_ex_role lb ρlg lb' (LM := lib_model lib_gs)) as [? STEP].
-      { eexists. split; [apply LIB_STEP| ]. done. }
-    eapply ls_mapping_tmap_corr in STEP as (?&?&?). rewrite H1. set_solver. } 
+  (*   assert (ls_tmap lb !! ρlg ≠ Some ∅) as TM_NE. *)
+  (*   { edestruct (locale_trans_ex_role lb ρlg lb' (LM := lib_model lib_gs)) as [? STEP]. *)
+  (*     { eexists. split; [apply LIB_STEP| ]. done. } *)
+  (*   eapply ls_mapping_tmap_corr in STEP as (?&?&?). rewrite H1. set_solver. }  *)
     
-    repeat erewrite @decide_False; try done. 
-    iSplitR.
-    - iPureIntro.  set_solver.
-    - rewrite dom_singleton_L big_sepS_singleton.
-      rewrite lookup_singleton.
-      iDestruct "FUEL" as (?) "[%EQ ?]". inversion EQ. subst.
-      iExists _. iFrame. iPureIntro. lia.
-  Qed.
+  (*   repeat erewrite @decide_False; try done.  *)
+  (*   iSplitR. *)
+  (*   - iPureIntro.  set_solver. *)
+  (*   - rewrite dom_singleton_L big_sepS_singleton. *)
+  (*     rewrite lookup_singleton. *)
+  (*     iDestruct "FUEL" as (?) "[%EQ ?]". inversion EQ. subst. *)
+  (*     iExists _. iFrame. iPureIntro. lia. *)
+  (* Qed. *)
 
-  Lemma lib_fuel_drop_step_preserves_LSI s rem:
-    fuel_drop_preserves_LSI s rem (LSI := LSI_groups_fixed lib_gs (M := lib_model_impl)).
-  Proof. 
-    (* done. *)
-    red. intros. red. rewrite dom_fmap. apply H0. 
-  Qed. 
+  (* Lemma lib_fuel_drop_step_preserves_LSI s rem: *)
+  (*   fuel_drop_preserves_LSI s rem (LSI := LSI_groups_fixed lib_gs (M := lib_model_impl)). *)
+  (* Proof.  *)
+  (*   (* done. *) *)
+  (*   red. intros. red. rewrite dom_fmap. apply H0.  *)
+  (* Qed.  *)
     
 
-  Lemma fuel_drop_step_lifting `{clientGS Σ} Einvs (DISJ_INV: Einvs ## ↑Ns):
-  LSG Einvs ∗ client_inv ⊢
-  ∀ (extr : execution_trace heap_lang) (auxtr : auxiliary_trace M)
-    (c2 : cfg heap_lang) s (fs : gmap (fmrole lib_model_impl) nat)
-    rem
-    (ζ : locale heap_lang) (_ : dom fs ≠ ∅)
+  (* Lemma fuel_drop_step_lifting `{clientGS Σ} Einvs (DISJ_INV: Einvs ## ↑Ns): *)
+  (* LSG Einvs ∗ client_inv ⊢ *)
+  (* ∀ (extr : execution_trace heap_lang) (auxtr : auxiliary_trace M) *)
+  (*   (c2 : cfg heap_lang) s (fs : gmap (fmrole lib_model_impl) nat) *)
+  (*   rem *)
+  (*   (ζ : locale heap_lang) (_ : dom fs ≠ ∅) *)
 
-    (_: (live_roles _ s) ∩ rem = ∅)
-    (_: rem ⊆ dom fs)
-    (_ : locale_step (trace_last extr) (Some ζ) c2),
-    has_fuels ζ (S <$> fs) (PMPP := lib_PMPP) -∗
-    partial_model_is s -∗
-    em_msi (trace_last extr) (trace_last auxtr) (em_GS0 := heap_fairnessGS)
-    ={Einvs ∪ ↑Ns}=∗
-    ∃ (δ2 : M) (ℓ : mlabel M),
-      ⌜em_valid_state_evolution_fairness (extr :tr[ Some ζ ]: c2)
-         (auxtr :tr[ ℓ ]: δ2)⌝ ∗
-      has_fuels ζ (filter (λ '(k, _), k ∈ dom fs ∖ rem) fs) (PMPP := lib_PMPP) ∗
-      partial_model_is s ∗
-      em_msi c2 δ2 (em_GS0 := heap_fairnessGS).
-  Proof.
-    iIntros "[#PMP #COMP]". iIntros "* FUELS_LIB ST_LIB MSI". simpl in *.
+  (*   (_: (live_roles _ s) ∩ rem = ∅) *)
+  (*   (_: rem ⊆ dom fs) *)
+  (*   (_ : locale_step (trace_last extr) (Some ζ) c2), *)
+  (*   has_fuels ζ (S <$> fs) (PMPP := lib_PMPP) -∗ *)
+  (*   partial_model_is s -∗ *)
+  (*   em_msi (trace_last extr) (trace_last auxtr) (em_GS0 := heap_fairnessGS) *)
+  (*   ={Einvs ∪ ↑Ns}=∗ *)
+  (*   ∃ (δ2 : M) (ℓ : mlabel M), *)
+  (*     ⌜em_valid_state_evolution_fairness (extr :tr[ Some ζ ]: c2) *)
+  (*        (auxtr :tr[ ℓ ]: δ2)⌝ ∗ *)
+  (*     has_fuels ζ (filter (λ '(k, _), k ∈ dom fs ∖ rem) fs) (PMPP := lib_PMPP) ∗ *)
+  (*     partial_model_is s ∗ *)
+  (*     em_msi c2 δ2 (em_GS0 := heap_fairnessGS). *)
+  (* Proof. *)
+  (*   iIntros "[#PMP #COMP]". iIntros "* FUELS_LIB ST_LIB MSI". simpl in *. *)
     
-    assert (S <$> fs ≠ ∅) as NE.
-    { intros ?%dom_empty_iff. set_solver. }
+  (*   assert (S <$> fs ≠ ∅) as NE. *)
+  (*   { intros ?%dom_empty_iff. set_solver. } *)
 
-    iPoseProof (lib_open_inv with "[$] FUELS_LIB") as "INV'"; [set_solver| ].
-    rewrite union_comm_L.
-    iMod (fupd_mask_frame_r _ _ Einvs with "INV'") as
-      "(-> & (%lb & ST & inv') & LM & YST_AUTH & (%f & Ff & %BOUND) & MAP & FR & YST & FUEL_LIB & CLOS)"; [set_solver| ].
+  (*   iPoseProof (lib_open_inv with "[$] FUELS_LIB") as "INV'"; [set_solver| ]. *)
+  (*   rewrite union_comm_L. *)
+  (*   iMod (fupd_mask_frame_r _ _ Einvs with "INV'") as *)
+  (*     "(-> & (%lb & ST & inv') & LM & YST_AUTH & (%f & Ff & %BOUND) & MAP & FR & YST & FUEL_LIB & CLOS)"; [set_solver| ]. *)
 
-    iAssert (⌜ s = ls_under lb ⌝)%I as %->.
-    { rewrite /model_state_interp.
-      iDestruct "inv'" as (?)"(?&?&?&ST_LIB'&?)".
-      (* TODO: make a lemma? *)
-      by iDestruct (own_valid_2 with "ST_LIB' ST_LIB") as
-      %[Heq%Excl_included%leibniz_equiv ?]%auth_both_valid_discrete. }
+  (*   iAssert (⌜ s = ls_under lb ⌝)%I as %->. *)
+  (*   { rewrite /model_state_interp. *)
+  (*     iDestruct "inv'" as (?)"(?&?&?&ST_LIB'&?)". *)
+  (*     (* TODO: make a lemma? *) *)
+  (*     by iDestruct (own_valid_2 with "ST_LIB' ST_LIB") as *)
+  (*     %[Heq%Excl_included%leibniz_equiv ?]%auth_both_valid_discrete. } *)
       
       
-    iMod (actual_update_no_step_enough_fuel_drop with "[LM FUEL_LIB] ST_LIB inv'") as (lb') "(%LIB_STEP & FUELS_LIB & ST_LIB & MSI_LIB & %TMAP_LIB)".
-    (* 3: { apply empty_subseteq. } *)
-    { eauto. }
-    4: { rewrite /has_fuels_S. rewrite has_fuels_equiv. iFrame.
-         iApply frag_fuel_is_big_sepM; done. }
-    2: { eauto. }
-    { done. }
-    { apply lib_fuel_drop_step_preserves_LSI. }
+  (*   iMod (actual_update_no_step_enough_fuel_drop with "[LM FUEL_LIB] ST_LIB inv'") as (lb') "(%LIB_STEP & FUELS_LIB & ST_LIB & MSI_LIB & %TMAP_LIB)". *)
+  (*   (* 3: { apply empty_subseteq. } *) *)
+  (*   { eauto. } *)
+  (*   4: { rewrite /has_fuels_S. rewrite has_fuels_equiv. iFrame. *)
+  (*        iApply frag_fuel_is_big_sepM; done. } *)
+  (*   2: { eauto. } *)
+  (*   { done. } *)
+  (*   { apply lib_fuel_drop_step_preserves_LSI. } *)
     
-    destruct (trace_last extr) as (σ1, tp1) eqn:LASTE. destruct c2 as (σ2, tp2).
-    rewrite LASTE.
-    (* rewrite difference_empty_L. *)
-    (* rewrite difference_empty_L in TMAP_LIB. *)
-    iAssert (has_fuels 0 {[ ρ_lib := f ]}) with "[MAP Ff]" as "FUELS".
-    { rewrite /has_fuels. rewrite dom_singleton_L big_sepS_singleton.
-      rewrite lookup_singleton. iFrame. iExists _. iFrame. done. }
+  (*   destruct (trace_last extr) as (σ1, tp1) eqn:LASTE. destruct c2 as (σ2, tp2). *)
+  (*   rewrite LASTE. *)
+  (*   (* rewrite difference_empty_L. *) *)
+  (*   (* rewrite difference_empty_L in TMAP_LIB. *) *)
+  (*   iAssert (has_fuels 0 {[ ρ_lib := f ]}) with "[MAP Ff]" as "FUELS". *)
+  (*   { rewrite /has_fuels. rewrite dom_singleton_L big_sepS_singleton. *)
+  (*     rewrite lookup_singleton. iFrame. iExists _. iFrame. done. } *)
 
-    rewrite -LASTE.
-    iPoseProof (update_client_state with "[$] [$] [$] [$] [$]") as "EM_STEP"; eauto.
-    { eexists. split; [apply LIB_STEP| ]. done. }
-    { lia. }
-    iMod (fupd_mask_mono with "EM_STEP") as (δ2 ℓ) "(EV & MSI & FUELS & ST & FR)"; [set_solver| ].
-    do 2 iExists _. iFrame "EV MSI".
+  (*   rewrite -LASTE. *)
+  (*   iPoseProof (update_client_state with "[$] [$] [$] [$] [$]") as "EM_STEP"; eauto. *)
+  (*   { eexists. split; [apply LIB_STEP| ]. done. } *)
+  (*   { lia. } *)
+  (*   iMod (fupd_mask_mono with "EM_STEP") as (δ2 ℓ) "(EV & MSI & FUELS & ST & FR)"; [set_solver| ]. *)
+  (*   do 2 iExists _. iFrame "EV MSI". *)
 
-    iDestruct ("CLOS" with "[ST MSI_LIB YST_AUTH]") as "CLOS".
-    { iNext. iExists (_, _). rewrite /client_inv_impl. iFrame. }
-    iMod (fupd_mask_frame_r _ _ Einvs with "CLOS") as "_"; [set_solver| ].
+  (*   iDestruct ("CLOS" with "[ST MSI_LIB YST_AUTH]") as "CLOS". *)
+  (*   { iNext. iExists (_, _). rewrite /client_inv_impl. iFrame. } *)
+  (*   iMod (fupd_mask_frame_r _ _ Einvs with "CLOS") as "_"; [set_solver| ]. *)
 
-    iModIntro.
-    iDestruct "FUELS" as "[MAP FUEL]". iDestruct "FUELS_LIB" as "[MAP_LIB FUELS_LIB]".
+  (*   iModIntro. *)
+  (*   iDestruct "FUELS" as "[MAP FUEL]". iDestruct "FUELS_LIB" as "[MAP_LIB FUELS_LIB]". *)
 
-    iFrame "ST_LIB". 
-    iSplitR "FUELS_LIB".
-    2: { rewrite dom_domain_restrict; [| set_solver]. done. }
-    simpl. rewrite dom_domain_restrict; [| set_solver].
-    rewrite /lib_pmi. do 3 iExists _. iFrame.
-    iSplitR; [done| ].
+  (*   iFrame "ST_LIB".  *)
+  (*   iSplitR "FUELS_LIB". *)
+  (*   2: { rewrite dom_domain_restrict; [| set_solver]. done. } *)
+  (*   simpl. rewrite dom_domain_restrict; [| set_solver]. *)
+  (*   rewrite /lib_pmi. do 3 iExists _. iFrame. *)
+  (*   iSplitR; [done| ]. *)
 
-    rewrite TMAP_LIB. rewrite lookup_insert.
-    destruct (decide (dom fs = rem)).
-    2: { 
+  (*   rewrite TMAP_LIB. rewrite lookup_insert. *)
+  (*   destruct (decide (dom fs = rem)). *)
+  (*   2: {  *)
 
-    iLeft.
-    iSplitR.
-    { iPureIntro. intros ?. apply n. set_solver. } 
-    (* rewrite lookup_insert. *)
-    repeat erewrite @decide_False with (P := (Some (dom fs ∖ rem) = Some ∅)).
-    (* 2-3: by intros [=]. *)
-    2, 3: intros [=]; set_solver. 
-    iSplitR.
-    { iPureIntro. set_solver. }
-    rewrite dom_singleton_L big_sepS_singleton.
-    rewrite lookup_singleton.
-    iDestruct "FUEL" as (?) "[%EQ ?]". inversion EQ. subst.
-    iExists _. iFrame. iPureIntro. lia. }
+  (*   iLeft. *)
+  (*   iSplitR. *)
+  (*   { iPureIntro. intros ?. apply n. set_solver. }  *)
+  (*   (* rewrite lookup_insert. *) *)
+  (*   repeat erewrite @decide_False with (P := (Some (dom fs ∖ rem) = Some ∅)). *)
+  (*   (* 2-3: by intros [=]. *) *)
+  (*   2, 3: intros [=]; set_solver.  *)
+  (*   iSplitR. *)
+  (*   { iPureIntro. set_solver. } *)
+  (*   rewrite dom_singleton_L big_sepS_singleton. *)
+  (*   rewrite lookup_singleton. *)
+  (*   iDestruct "FUEL" as (?) "[%EQ ?]". inversion EQ. subst. *)
+  (*   iExists _. iFrame. iPureIntro. lia. } *)
     
-    subst rem. iRight. iSplitR.
-    { iPureIntro. set_solver. }
-    rewrite difference_diag_L. repeat erewrite decide_True.
-    2, 3: done.
-    iSplitR.
-    { iPureIntro. set_solver. }
-    rewrite dom_singleton_L big_sepS_singleton.
-    rewrite lookup_singleton.
-    iDestruct "FUEL" as (?) "[%EQ ?]". inversion EQ.
-    iFrame.         
-  Qed.
+  (*   subst rem. iRight. iSplitR. *)
+  (*   { iPureIntro. set_solver. } *)
+  (*   rewrite difference_diag_L. repeat erewrite decide_True. *)
+  (*   2, 3: done. *)
+  (*   iSplitR. *)
+  (*   { iPureIntro. set_solver. } *)
+  (*   rewrite dom_singleton_L big_sepS_singleton. *)
+  (*   rewrite lookup_singleton. *)
+  (*   iDestruct "FUEL" as (?) "[%EQ ?]". inversion EQ. *)
+  (*   iFrame.          *)
+  (* Qed. *)
 
 
-  Lemma lib_model_step_preserves_LSI:
-  ∀ (s1 : lib_model_impl) (ρ : fmrole lib_model_impl) 
-    (s2 : lib_model_impl) (fs1 fs2 : gmap (fmrole lib_model_impl) nat),
-    model_step_preserves_LSI s1 ρ s2 fs1 fs2 (LSI := LSI_groups_fixed lib_gs).
-  Proof.
-    (* can be proven trivially, but the proof below should work for non-trivial Gs *)
-    intros. red. intros * LSI1 STEP INρ. red. intros g' DOMg'.
-    apply LSI1.
-    rewrite dom_insert_L in DOMg'.
-    apply elem_of_union in DOMg' as [IN| ?]; [| done].
-    apply elem_of_singleton in IN as ->.
-    eapply @elem_of_dom; [by apply _| ].
-    destruct (R !! g) eqn:RG; done. 
-  Qed.
+  (* Lemma lib_model_step_preserves_LSI: *)
+  (* ∀ (s1 : lib_model_impl) (ρ : fmrole lib_model_impl)  *)
+  (*   (s2 : lib_model_impl) (fs1 fs2 : gmap (fmrole lib_model_impl) nat), *)
+  (*   model_step_preserves_LSI s1 ρ s2 fs1 fs2 (LSI := LSI_groups_fixed lib_gs). *)
+  (* Proof. *)
+  (*   (* can be proven trivially, but the proof below should work for non-trivial Gs *) *)
+  (*   intros. red. intros * LSI1 STEP INρ. red. intros g' DOMg'. *)
+  (*   apply LSI1. *)
+  (*   rewrite dom_insert_L in DOMg'. *)
+  (*   apply elem_of_union in DOMg' as [IN| ?]; [| done]. *)
+  (*   apply elem_of_singleton in IN as ->. *)
+  (*   eapply @elem_of_dom; [by apply _| ]. *)
+  (*   destruct (R !! g) eqn:RG; done.  *)
+  (* Qed. *)
     
-  Lemma model_step_lifting `{clientGS Σ} Einvs (DISJ_INV: Einvs ## ↑Ns):
-  LSG Einvs ∗ client_inv ⊢
-  ∀ (extr : execution_trace heap_lang) (auxtr : auxiliary_trace M)
-    (tp1 tp2 : list (language.expr heap_lang)) (σ1 σ2 : language.state heap_lang)
-    (s1 s2 : lib_model_impl) (fs1 fs2 : gmap (fmrole lib_model_impl) nat)
-    (ρ : fmrole lib_model_impl) (δ1 : M) (ζ : locale heap_lang)
-    (fr1 fr_stash : gset (fmrole lib_model_impl))
-    (_ : live_roles lib_model_impl s2 ∖ live_roles lib_model_impl s1 ⊆ fr1 ∪ dom fs1 ∩ dom fs2)
-    (_ : fr_stash ⊆ dom fs1) (_ : live_roles lib_model_impl s1
-                                  ∩ (fr_stash ∖ {[ρ]}) = ∅)
-    (_ : dom fs2 ∩ fr_stash = ∅) (_ : trace_last extr = (tp1, σ1))
-    (_ : trace_last auxtr = δ1) (_ : locale_step (tp1, σ1) (Some ζ) (tp2, σ2))
-    (_ : fmtrans lib_model_impl s1 (Some ρ) s2)
-    (_ : valid_new_fuelmap fs1 fs2 s1 s2 ρ (LM := lib_model lib_gs))
-  ,
-    has_fuels ζ fs1 (PMPP := lib_PMPP) -∗
-    partial_model_is s1 (PartialModelPredicatesPre := lib_PMPP) -∗
-    em_msi (tp1, σ1) δ1 (em_GS0 := heap_fairnessGS) -∗
-    partial_free_roles_are fr1 (PartialModelPredicatesPre := lib_PMPP)
-    ={Einvs ∪ ↑Ns}=∗
-    ∃ (δ2 : M) (ℓ : mlabel M),
-      ⌜em_valid_state_evolution_fairness (extr :tr[ Some ζ ]: (tp2, σ2))
-         (auxtr :tr[ ℓ ]: δ2)⌝ ∗
-      has_fuels ζ fs2 (PMPP := lib_PMPP) ∗
-      partial_model_is s2 (PartialModelPredicatesPre := lib_PMPP) ∗
-      em_msi (tp2, σ2) δ2 (em_GS0 := heap_fairnessGS) ∗
-      partial_free_roles_are
-        (fr1 ∖ (live_roles lib_model_impl s2 ∖ (live_roles lib_model_impl s1 ∪ dom fs1 ∩ dom fs2))
-         ∪ fr_stash) (PartialModelPredicatesPre := lib_PMPP).
-  Proof.
-    iIntros "[#PMP #COMP]". iIntros "* FUELS_LIB ST_LIB MSI FR_LIB". simpl in *.
+  (* Lemma model_step_lifting `{clientGS Σ} Einvs (DISJ_INV: Einvs ## ↑Ns): *)
+  (* LSG Einvs ∗ client_inv ⊢ *)
+  (* ∀ (extr : execution_trace heap_lang) (auxtr : auxiliary_trace M) *)
+  (*   (tp1 tp2 : list (language.expr heap_lang)) (σ1 σ2 : language.state heap_lang) *)
+  (*   (s1 s2 : lib_model_impl) (fs1 fs2 : gmap (fmrole lib_model_impl) nat) *)
+  (*   (ρ : fmrole lib_model_impl) (δ1 : M) (ζ : locale heap_lang) *)
+  (*   (fr1 fr_stash : gset (fmrole lib_model_impl)) *)
+  (*   (_ : live_roles lib_model_impl s2 ∖ live_roles lib_model_impl s1 ⊆ fr1 ∪ dom fs1 ∩ dom fs2) *)
+  (*   (_ : fr_stash ⊆ dom fs1) (_ : live_roles lib_model_impl s1 *)
+  (*                                 ∩ (fr_stash ∖ {[ρ]}) = ∅) *)
+  (*   (_ : dom fs2 ∩ fr_stash = ∅) (_ : trace_last extr = (tp1, σ1)) *)
+  (*   (_ : trace_last auxtr = δ1) (_ : locale_step (tp1, σ1) (Some ζ) (tp2, σ2)) *)
+  (*   (_ : fmtrans lib_model_impl s1 (Some ρ) s2) *)
+  (*   (_ : valid_new_fuelmap fs1 fs2 s1 s2 ρ (LM := lib_model lib_gs)) *)
+  (* , *)
+  (*   has_fuels ζ fs1 (PMPP := lib_PMPP) -∗ *)
+  (*   partial_model_is s1 (PartialModelPredicatesPre := lib_PMPP) -∗ *)
+  (*   em_msi (tp1, σ1) δ1 (em_GS0 := heap_fairnessGS) -∗ *)
+  (*   partial_free_roles_are fr1 (PartialModelPredicatesPre := lib_PMPP) *)
+  (*   ={Einvs ∪ ↑Ns}=∗ *)
+  (*   ∃ (δ2 : M) (ℓ : mlabel M), *)
+  (*     ⌜em_valid_state_evolution_fairness (extr :tr[ Some ζ ]: (tp2, σ2)) *)
+  (*        (auxtr :tr[ ℓ ]: δ2)⌝ ∗ *)
+  (*     has_fuels ζ fs2 (PMPP := lib_PMPP) ∗ *)
+  (*     partial_model_is s2 (PartialModelPredicatesPre := lib_PMPP) ∗ *)
+  (*     em_msi (tp2, σ2) δ2 (em_GS0 := heap_fairnessGS) ∗ *)
+  (*     partial_free_roles_are *)
+  (*       (fr1 ∖ (live_roles lib_model_impl s2 ∖ (live_roles lib_model_impl s1 ∪ dom fs1 ∩ dom fs2)) *)
+  (*        ∪ fr_stash) (PartialModelPredicatesPre := lib_PMPP). *)
+  (* Proof. *)
+  (*   iIntros "[#PMP #COMP]". iIntros "* FUELS_LIB ST_LIB MSI FR_LIB". simpl in *. *)
     
-    assert (ρ ∈ dom fs1) as DOM1ρ by apply x7.
-    assert (dom fs1 ≠ ∅ /\ fs1 ≠ ∅) as [FS1nz FS1nz'].
-    { split; intros ?; set_solver. }
+  (*   assert (ρ ∈ dom fs1) as DOM1ρ by apply x7. *)
+  (*   assert (dom fs1 ≠ ∅ /\ fs1 ≠ ∅) as [FS1nz FS1nz']. *)
+  (*   { split; intros ?; set_solver. } *)
     
-    iPoseProof (lib_open_inv with "[$] FUELS_LIB") as "INV'"; [done| ].
-    rewrite union_comm_L.
-    iMod (fupd_mask_frame_r _ _ Einvs with "INV'") as
-      "(-> & (%lb & ST & inv') & LM & YST_AUTH & (%f & Ff & %BOUND) & MAP & FR & YST & FUEL_LIB & CLOS)"; [set_solver| ].
+  (*   iPoseProof (lib_open_inv with "[$] FUELS_LIB") as "INV'"; [done| ]. *)
+  (*   rewrite union_comm_L. *)
+  (*   iMod (fupd_mask_frame_r _ _ Einvs with "INV'") as *)
+  (*     "(-> & (%lb & ST & inv') & LM & YST_AUTH & (%f & Ff & %BOUND) & MAP & FR & YST & FUEL_LIB & CLOS)"; [set_solver| ]. *)
 
-    iPoseProof (LM_steps_gen_nofork_sub with "PMP") as "PMP'".
-    iMod (actual_update_step_still_alive_gen with "[LM FUEL_LIB] [$] [$] [$]") as "LIFT"; eauto.
-    2: { rewrite has_fuels_equiv. iFrame. iApply frag_fuel_is_big_sepM; done. }
-    { apply lib_model_step_preserves_LSI. }
+  (*   iPoseProof (LM_steps_gen_nofork_sub with "PMP") as "PMP'". *)
+  (*   iMod (actual_update_step_still_alive_gen with "[LM FUEL_LIB] [$] [$] [$]") as "LIFT"; eauto. *)
+  (*   2: { rewrite has_fuels_equiv. iFrame. iApply frag_fuel_is_big_sepM; done. } *)
+  (*   { apply lib_model_step_preserves_LSI. } *)
 
-    iDestruct "LIFT" as (lb') "(%LIB_STEP & FUELS_LIB & ST_LIB & MSI_LIB & FR_LIB & %TMAP_LIB)".
-    simpl. iFrame "ST_LIB".
+  (*   iDestruct "LIFT" as (lb') "(%LIB_STEP & FUELS_LIB & ST_LIB & MSI_LIB & FR_LIB & %TMAP_LIB)". *)
+  (*   simpl. iFrame "ST_LIB". *)
     
-    iAssert (has_fuels 0 {[ ρ_lib := f ]}) with "[MAP Ff]" as "FUELS".
-    { rewrite /has_fuels. rewrite dom_singleton_L big_sepS_singleton.
-      rewrite lookup_singleton. iFrame. iExists _. iFrame. done. }
+  (*   iAssert (has_fuels 0 {[ ρ_lib := f ]}) with "[MAP Ff]" as "FUELS". *)
+  (*   { rewrite /has_fuels. rewrite dom_singleton_L big_sepS_singleton. *)
+  (*     rewrite lookup_singleton. iFrame. iExists _. iFrame. done. } *)
 
-    rewrite -x3 -x4. rewrite -x3 in x5.
-    iPoseProof (update_client_state with "[$] [MSI] [ST] [$] [$]") as "EM_STEP"; eauto.
-    { eexists. split; [apply LIB_STEP| ]. done. }
-    { lia. }
-    iMod (fupd_mask_mono with "EM_STEP") as (δ2 ℓ) "(EV & MSI & FUELS & ST & FR)"; [set_solver| ].
-    do 2 iExists _. iFrame "EV MSI".
+  (*   rewrite -x3 -x4. rewrite -x3 in x5. *)
+  (*   iPoseProof (update_client_state with "[$] [MSI] [ST] [$] [$]") as "EM_STEP"; eauto. *)
+  (*   { eexists. split; [apply LIB_STEP| ]. done. } *)
+  (*   { lia. } *)
+  (*   iMod (fupd_mask_mono with "EM_STEP") as (δ2 ℓ) "(EV & MSI & FUELS & ST & FR)"; [set_solver| ]. *)
+  (*   do 2 iExists _. iFrame "EV MSI". *)
 
-    iDestruct ("CLOS" with "[ST MSI_LIB YST_AUTH]") as "CLOS".
-    { iNext. iExists (_, _). rewrite /client_inv_impl. iFrame. }
-    iMod (fupd_mask_frame_r _ _ Einvs with "CLOS") as "_"; [set_solver| ].
-    iModIntro.
+  (*   iDestruct ("CLOS" with "[ST MSI_LIB YST_AUTH]") as "CLOS". *)
+  (*   { iNext. iExists (_, _). rewrite /client_inv_impl. iFrame. } *)
+  (*   iMod (fupd_mask_frame_r _ _ Einvs with "CLOS") as "_"; [set_solver| ]. *)
+  (*   iModIntro. *)
 
-    rewrite !has_fuels_equiv. simpl.
-    iDestruct "FUELS" as "[MAP FUELS]".
-    iDestruct "FUELS_LIB" as "[MAP' FUELS_LIB]". iFrame "FUELS_LIB FR_LIB".
-    rewrite /lib_pmi. do 3 iExists _. iFrame.
-    iSplitR; [done |].
-    rewrite TMAP_LIB. rewrite lookup_insert.
-    dEq.
-    - iRight. rewrite big_sepM_singleton. iFrame.
-      iPureIntro. set_solver.
-    - iLeft. rewrite big_sepM_singleton.
-      iApply bi.sep_assoc. iSplitR "FUELS".
-      2: { iExists _. iFrame. iPureIntro. lia. }
-      iPureIntro. split; [| set_solver]. intros ?. rewrite H1 in n. done.
-  Qed.
+  (*   rewrite !has_fuels_equiv. simpl. *)
+  (*   iDestruct "FUELS" as "[MAP FUELS]". *)
+  (*   iDestruct "FUELS_LIB" as "[MAP' FUELS_LIB]". iFrame "FUELS_LIB FR_LIB". *)
+  (*   rewrite /lib_pmi. do 3 iExists _. iFrame. *)
+  (*   iSplitR; [done |]. *)
+  (*   rewrite TMAP_LIB. rewrite lookup_insert. *)
+  (*   dEq. *)
+  (*   - iRight. rewrite big_sepM_singleton. iFrame. *)
+  (*     iPureIntro. set_solver. *)
+  (*   - iLeft. rewrite big_sepM_singleton. *)
+  (*     iApply bi.sep_assoc. iSplitR "FUELS". *)
+  (*     2: { iExists _. iFrame. iPureIntro. lia. } *)
+  (*     iPureIntro. split; [| set_solver]. intros ?. rewrite H1 in n. done. *)
+  (* Qed. *)
 
 
   Lemma lib_PMP `{clientGS Σ} Einvs (DISJ_INV: Einvs ## ↑Ns):
     LSG Einvs ∗ client_inv ⊢
     (* PartialModelPredicates (Einvs ∪ ↑Ns) (LM := LM) (iLM := spinlock_model) (PMPP := (sl1_PMPP γ)).  *)
-    LM_steps_gen_nofork (Einvs ∪ ↑Ns) (EM := EM) (iLM := lib_model lib_gs) (PMPP := lib_PMPP) (eGS := heap_fairnessGS).
+    LM_steps_gen_nofork (Einvs ∪ ↑Ns) (EM := EM) (iLM := lib_model lib_gs) (PMPP := lib_PMPP) (eGS := heap_fairnessGS) (relies_on := relies_on_lib).
   Proof.
-    iIntros "[#PMP #COMP]". iApply @Build_LM_steps_gen_nofork.
+    (* iIntros "[#PMP #COMP]". iApply @Build_LM_steps_gen_nofork. *)
 
-    iModIntro. repeat iSplitR.
-    - iIntros "* FUELS_LIB ST MSI".
-      iDestruct (fuel_drop_step_lifting with "[$] [] [] [] [] FUELS_LIB ST MSI") as "LIFT"; eauto.
-      (* change the PMP interface so it allows fupd in fuel step *)
-      admit.      
-    - iIntros "* FUELS_LIB MSI".
-      iDestruct (fuel_keep_step_lifting with "[$] [] [] FUELS_LIB MSI") as "LIFT"; eauto.
-      (* same as above *)
-      admit.
-    - iIntros "* FUELS_LIB ST MSI FR".
-      iApply (model_step_lifting with "[$] [] [] [] [] [] [] [] [] [] [$] [$] [$] [$]"); eauto.
+    (* iModIntro. repeat iSplitR. *)
+    (* - iIntros "* FUELS_LIB ST MSI". *)
+    (*   iDestruct (fuel_drop_step_lifting with "[$] [] [] [] [] FUELS_LIB ST MSI") as "LIFT"; eauto. *)
+    (*   (* change the PMP interface so it allows fupd in fuel step *) *)
+    (*   admit.       *)
+    (* - iIntros "* FUELS_LIB MSI". *)
+    (*   iDestruct (fuel_keep_step_lifting with "[$] [] [] FUELS_LIB MSI") as "LIFT"; eauto. *)
+    (*   (* same as above *) *)
+    (*   admit. *)
+    (* - iIntros "* FUELS_LIB ST MSI FR". *)
+    (*   iApply (model_step_lifting with "[$] [] [] [] [] [] [] [] [] [] [$] [$] [$] [$]"); eauto. *)
+
   Admitted.
-
 
 End LibPMP. 
