fairness/examples/comp/tracker.v
@@ -1,0 +1,62 @@
+From iris.base_logic.lib Require Import invariants.
+From iris.algebra Require Import excl_auth numbers gset csum. 
+From iris.proofmode Require Import tactics.
+
+
+Section TrackerRA.
+
+  Definition trackerRA: ucmra := excl_authR boolO. 
+  
+  Definition tr_tracked: bool := true.
+  Definition tr_free: bool := false.
+
+  (***********)
+  
+  Context `{inG Σ trackerRA}.   
+  
+  Definition tracked (γ: gname) (P: iProp Σ): iProp Σ :=
+    own γ (●E tr_tracked) ∗ P ∨ own γ (●E tr_free).
+
+  Lemma init_tracker (P: iProp Σ): 
+    ⊢ (|==> ∃ γ, tracked γ P ∗ own γ (◯E tr_free))%I.
+  Proof.
+    iStartProof. 
+    iMod (own_alloc (●E tr_free  ⋅ ◯E tr_free)) as (γ) "[AUTH FRAG]".
+    { apply auth_both_valid_2; eauto. by compute. }
+    iModIntro. iExists _. iFrame.
+  Qed. 
+
+  Lemma start_tracking γ (P: iProp Σ):
+    ⊢ (own γ (◯E tr_free) ∗ P ∗ tracked γ P ==∗ own γ (◯E tr_tracked) ∗ tracked γ P)%I.
+  Proof.
+    iIntros "(FRAG & P & [[AUTH ?] | AUTH])".
+    { iDestruct (own_op with "[FRAG AUTH]") as "O"; [by iFrame| ].
+      iDestruct (own_valid with "O") as "%V".      
+      eapply excl_auth_agree in V. done. } 
+
+    iMod (own_update with "[AUTH FRAG]") as "OWN". 
+    { eapply excl_auth_update. }
+    { iApply own_op. iFrame. }
+    iDestruct "OWN" as "[AUTH FRAG]". 
+    
+    iModIntro. iFrame. iLeft. iFrame.
+  Qed. 
+
+  Lemma stop_tracking γ (P: iProp Σ):
+    ⊢ (own γ (◯E tr_tracked) ∗ tracked γ P ==∗ own γ (◯E tr_free) ∗ P ∗ tracked γ P)%I.
+  Proof.
+    iIntros "(FRAG & [[AUTH ?] | AUTH])".
+    2: { iDestruct (own_op with "[FRAG AUTH]") as "O"; [by iFrame| ].
+         iDestruct (own_valid with "O") as "%V".      
+         eapply excl_auth_agree in V. done. }
+
+    iMod (own_update with "[AUTH FRAG]") as "OWN". 
+    { eapply excl_auth_update. }
+    { iApply own_op. iFrame. }
+    iDestruct "OWN" as "[AUTH FRAG]". 
+    
+    iModIntro. iFrame.
+  Qed. 
+  
+
+End TrackerRA.
